bedrock2/src/bedrock2Examples/swap.v
@@ -33,16 +33,23 @@ Section WithParameters.
   Context {word: word.word 32} {mem: map.map word Byte.byte}.
   Context {word_ok: word.ok word} {mem_ok: map.ok mem}.
 
+  Locate "program_logic_goal_for_function!". Print program_logic_goal_for.
+  Locate "fnct!". Print spec_of.
+
   Instance spec_of_swap : spec_of "swap" :=
     fnspec! "swap" a_addr b_addr / a b R,
     { requires t m := m =* scalar a_addr a * scalar b_addr b * R;
       ensures T M :=  M =* scalar a_addr b * scalar b_addr a * R /\ (filterio T) = (filterio t) }.
-
-  Lemma f (P : nat -> nat -> Prop) : (forall a b, P a b) -> exists x y, P x y.
-  Proof. intros H. exists O. exists O. apply H. Defined. Print f. Check ex_intro.
+  
+  Instance ct_swap : ct_proof_of "swap" :=
+      fnct! "swap" a_addr b_addr | (dummy1 : nat) / (dummy2 : nat) | a b R,
+      { requires t m := m =* scalar a_addr a * scalar b_addr b * R }.
 
   Lemma swap_ok : program_logic_goal_for_function! swap.
   Proof. repeat straightline; eauto. Qed.
+
+  Lemma swap_ct : program_logic_ct_goal_for_function! swap.
+  Proof. repeat straightline. Qed.
 
   Instance spec_of_bad_swap : spec_of "bad_swap" :=
     fnspec! "bad_swap" a_addr b_addr / a b R,
